notes.md
@@ -1,6 +1,106 @@
 https://xavierleroy.org/publi/validated-parser.pdf
 
 
+Definition Predicts extended extending :=
+  forall matched, MatchFrontAlign extending matched
+    -> MatchFrontAlign extended matched.
+Definition Prevents discriminant discriminated :=
+  forall matched, MatchFrontAlign discriminant matched
+    -> ~(MatchFrontAlign discriminated matched).
+
+
+
+
+there are three cases for a main/against:
+1. they are exactly equivalent: EqTotalAlign against main
+2. against extends main: EqExtends against main (lookahead = main)
+3. main extends against: EqExtends main against (EqDivergesAt lookahead against)
+4. they have a point of divergence: (EqDivergesAt lookahead against)
+
+the definition of DivergesAt makes 3 and 4 equivalent, but they have different consequences regarding prediction
+in 4, if lookahead (and therefore main) matches, then by construction against can't match since the tail of against doesn't align
+but in 3, it instead means that main (and lookahead!) is itself a lookahead for against
+
+or perhaps this is our situation for an inferred unless!!!
+in situation 3, merely testing for *main* to match could erroneously cause us to move forward and parse a shorter sequence when the longer sequence could match, so rather than emitting a mere lookahead for main, we emit a *negative* lookahead for against (and a minimal lookahead to test if we should enter main)
+
+
+
+
+main: A
+against: B
+lookahead: A
+lookahead = (firstn 1 main)
+EqDivergesAt :=
+  TotalAlign (firstn 0 against) (firstn 0 lookahead)
+  /\ Diverge (skipn 0 against) (skipn 0 lookahead)
+
+main: A B C
+against: A E
+lookahead: A B
+lookahead = (firstn 2 main)
+EqDivergesAt :=
+  TotalAlign (firstn 1 against) (firstn 1 lookahead)
+  /\ Diverge (skipn 1 against) (skipn 1 lookahead)
+
+main: A B
+against: A B C
+lookahead: A B
+lookahead = (firstn 2 main)
+EqDivergesAt :=
+  TotalAlign (firstn 1 against) (firstn 1 lookahead)
+  /\ Diverge (skipn 1 against) (skipn 1 lookahead)
+
+
+
+
+
+a correct lookahead is one that, for some nodes/node lists A and B
+- the lookahead head matches A
+- if a token stream would match A ++ B, then the lookahead will say yes
+- if a token stream would not match A ++ B (but only B?) then it will say no. probably that means that it simply *doesn't* match B??
+
+
+if the lookahead matches B, then it also must *totally* match A, implying that A is subsumed by B
+otherwise, it must not match B but only A
+this means there are two ways to construct evidence that a lookahead is correct
+- it matches A but not B
+- it matches A and B, but B subsumes A
+
+LookaheadCorrect L A B := forall stream, LookaheadYes L A B stream <-> NodeListMatches (A ++ B) stream
+
+
+
+
+
+If the stream is:
+
+- merely A, does the lookahead match? my first impulse is yes, although whether the *surrounding rule* will match is a much more fraught question
+-
+
+
+now it's all about how to define a "maximal" match
+that's what defines a correct lookahead, it will tell us whether to take the current option in such a way that the overall match we produce will be maximal
+now just what is maximal????
+
+
+
+let's say we have a rule like this that we need to generate lookaheads for
+what we really want to know is what lookahead do we need to test when we hit A B
+a consume is all or nothing
+(A B)? (A)
+
+the lookahead has to be (A B), since merely (A) would falsely enter the ? consume if the
+
+
+
+
+
+
+
+
+
+
 
 
 
@@ -55,7 +155,7 @@ https://xavierleroy.org/publi/validated-parser.pdf
 
 // in order to parse a statement, we need to generally know whether we're about to encounter a pattern or an array
 
-// it all comes down to those states in which what to do next isn't merely determined by what's in front o fus, but also what's behind us
+// it all comes down to those states in which what to do next isn't merely determined by what's in front of us, but also what's behind us
 
 
 
